theories/Base.v
@@ -219,7 +219,6 @@ Module Type BaseMixin (Import TY : Types).
       | exp_get_slice_int e => term_get_slice_int (seval_exp e)
       | exp_unsigned e     => term_unsigned (seval_exp e)
       | exp_truncate m e   => term_truncate m (seval_exp e)
-      | exp_extract s l e  => term_extract s l (seval_exp e)
       | exp_negate e       => term_negate (seval_exp e)
       | exp_list es        => term_list (List.map seval_exp es)
       | exp_bvec es        => term_bvec (Vector.map seval_exp es)
