theories/Symbolic/Propositions.v
@@ -1684,7 +1684,7 @@ Module Type SymPropOn
     | eterm_get_slice_int {n} (e : ETerm ty.int) : ETerm (ty.bvec n)
     | eterm_unsigned {n} (e : ETerm (ty.bvec n)) : ETerm ty.int
     | eterm_truncate {n} (m : nat) {p : IsTrue (m <=? n)} (e: ETerm (ty.bvec n)) : ETerm (ty.bvec m)
-    | eterm_extract {n} (s l : nat) (e : ETerm (ty.bvec n)) : ETerm (ty.bvec l)
+    | eterm_vector_subrange {n} (e : ETerm (ty.bvec n)) (s l : nat) {p : IsTrue (s + l <=? n)} : ETerm (ty.bvec l)
     | eterm_negate  {n} (e : ETerm (ty.bvec n)) : ETerm (ty.bvec n)
     | eterm_tuple   {σs : Ctx Ty} (ts : Env ETerm σs) : ETerm (ty.tuple σs)
     | eterm_union   {U : unioni} (K : unionk U) (t : ETerm (unionk_ty U K)) : ETerm (ty.union U)
@@ -1732,23 +1732,23 @@ Module Type SymPropOn
     Definition erase_term {Σ} : forall {σ} (t : Term Σ σ), ETerm σ :=
       fix erase {σ} t :=
         match t with
-        | @term_var _ ℓ σ ℓIn => eterm_var ℓ σ (ctx.in_at ℓIn)
-        | term_val σ v => eterm_val σ v
-        | term_binop op t1 t2 => eterm_binop op (erase t1) (erase t2)
-        | term_neg t => eterm_neg (erase t)
-        | term_not t => eterm_not (erase t)
-        | term_inl t => eterm_inl (erase t)
-        | term_inr t => eterm_inr (erase t)
-        | term_sext t => eterm_sext (erase t)
-        | term_zext t => eterm_zext (erase t)
-        | term_get_slice_int t => eterm_get_slice_int (erase t)
-        | term_unsigned t => eterm_unsigned (erase t)
-        | term_truncate m t => eterm_truncate m (erase t)
-        | term_extract s l t => eterm_extract s l (erase t)
-        | term_negate t => eterm_negate (erase t)
-        | term_tuple ts => eterm_tuple (env.map (fun _ => erase) ts)
-        | term_union U K t => eterm_union K (erase t)
-        | term_record R ts => eterm_record R (env.map (fun _ => erase) ts)
+        | @term_var _ ℓ σ ℓIn         => eterm_var ℓ σ (ctx.in_at ℓIn)
+        | term_val σ v               => eterm_val σ v
+        | term_binop op t1 t2        => eterm_binop op (erase t1) (erase t2)
+        | term_neg t                 => eterm_neg (erase t)
+        | term_not t                 => eterm_not (erase t)
+        | term_inl t                 => eterm_inl (erase t)
+        | term_inr t                 => eterm_inr (erase t)
+        | term_sext t                => eterm_sext (erase t)
+        | term_zext t                => eterm_zext (erase t)
+        | term_get_slice_int t       => eterm_get_slice_int (erase t)
+        | term_unsigned t            => eterm_unsigned (erase t)
+        | term_truncate m t          => eterm_truncate m (erase t)
+        | term_vector_subrange t s l => eterm_vector_subrange (erase t) s l 
+        | term_negate t              => eterm_negate (erase t)
+        | term_tuple ts              => eterm_tuple (env.map (fun _ => erase) ts)
+        | term_union U K t           => eterm_union K (erase t)
+        | term_record R ts           => eterm_record R (env.map (fun _ => erase) ts)
         end.
 
     Definition erase_formula {Σ} : Formula Σ -> EFormula :=
@@ -1851,8 +1851,8 @@ Module Type SymPropOn
             bv.unsigned <$> inst_eterm t0
         | @eterm_truncate _ m p t0 =>
             (fun v => bv.truncate m v) <$> inst_eterm t0
-        | @eterm_extract _ s l t0 =>
-            (fun v => bv.extract s l v) <$> inst_eterm t0
+        | @eterm_vector_subrange _ t0 s l _ =>
+            (fun v => bv.vector_subrange v s l) <$> inst_eterm t0
         | eterm_negate t0 =>
             bv.negate <$> inst_eterm t0
         | @eterm_tuple σs ts =>
